proof complete (TODO: k)

coq/two/LambdaTwo.v
@@ -1,3 +1,4 @@
+Require Import Program.Tactics.
 Require Export LambdaTwoSyntax.
 Require Export IndistinguishabilityTwo.
 Require Import LibTactics.
@@ -5,95 +6,42 @@ Require Import LibTactics.
 Fixpoint eval (L : two) (P : value -> value -> Prop)
          (pc : two) (e : env) (t : term) (k : nat) (a : atom)
          {struct k} : Prop :=
-  match t, k with
-    | TNat n, 0 =>
+  match t with
+    | TNat n =>
       a = Atom (VNat n) pc
-    | TVar n, 0 =>
-      match atIndex e n with
-        | Some (Atom v l) =>
-          a = Atom v (l ⊔ pc)
-        | None => False
-      end
-    | TAbs t', 0 =>
+    | TVar n =>
+      exists v l,
+        atIndex e n = Some (Atom v l) /\
+        a = Atom v (l ⊔ pc)
+    | TAbs t' =>
       a = Atom (VClos e t') pc
-    | TApp t1 t2, S k' =>
-      forall e1' t1' l1 a2 a3,
-        eval L P pc e t1 k' (Atom (VClos e1' t1') l1) ->
-        eval L P pc e t2 k' a2 ->
-        eval L P l1 (a2 :: e1') t1' k' a3 ->
-        a = a3
-    | TDecl t1 t2, S k' =>
-      forall e1' t1' l1 a2 v3 l3,
-        eval L P pc e t1 k' (Atom (VClos e1' t1') l1) ->
-        eval L P pc e t2 k' a2 ->
-        eval L P l1 (a2 :: e1') t1' k' (Atom v3 l3) ->
-        match l3 with
-          | Bottom2 =>
-            a = Atom v3 Bottom2
-          | Top2 =>
-            (forall a2' e2' v3',
-               env_LPequiv L P (a2 :: e1') (a2' :: e2') ->
-               eval L P l1 (a2' :: e2') t1' k' (Atom v3' Top2) ->
-               value_LPequiv L P v3 v3') ->
-            a = Atom v3 Bottom2
-        end
-    | _, _ => False
+    | TApp t1 t2 =>
+      match k with
+        | S k' =>
+          exists e1' t1' l1 a2 a3,
+            eval L P pc e t1 k' (Atom (VClos e1' t1') l1) /\
+            eval L P pc e t2 k' a2 /\
+            eval L P l1 (a2 :: e1') t1' k' a3 /\
+            a = a3
+        | 0 => False
+      end
+    | TDecl t1 t2 =>
+      match k with
+        | S k' =>
+          exists e1' t1' l1 a2 v3 l3,
+            eval L P pc e t1 k' (Atom (VClos e1' t1') l1) /\
+            eval L P pc e t2 k' a2 /\
+            eval L P l1 (a2 :: e1') t1' k' (Atom v3 l3) /\
+            match l3 with
+              | Bottom2 =>
+                a = Atom v3 Bottom2
+              | Top2 =>
+                (forall a2' e2' v3',
+                   env_LPequiv L P (a2 :: e1') (a2' :: e2') ->
+                   eval L P l1 (a2' :: e2') t1' k' (Atom v3' Top2) ->
+                   value_LPequiv L P v3 v3') /\
+                a = Atom v3 Bottom2
+            end
+        | 0 => False
+      end
   end.
-
-Lemma eval_nat_inv :
-  forall L P k pc e n a,
-    eval L P pc e (TNat n) k a ->
-    a = Atom (VNat n) pc.
-Proof.
-  introv Heval. destruct k; auto.
-Qed.
-
-Lemma eval_var_inv :
-  forall L P k pc e n a,
-    eval L P pc e (TVar n) k a ->
-    exists v l,
-      atIndex e n = Some (Atom v l) /\
-      a = Atom v (l ⊔ pc).
-Proof.
-  introv Heval. remember (atIndex e n) as o.
-  destruct o as [[v' l'] |]; destruct pc; destruct k;
-  unfold eval in Heval; try rewrite <- Heqo in Heval; inversion Heval;
-  apply ex_intro with v'; apply ex_intro with l'; auto.
-Qed.
-               
-Lemma eval_abs_inv :
-  forall L P k pc e t a,
-    eval L P pc e (TAbs t) k a ->
-    a = Atom (VClos e t) pc.
-Proof.
-  introv Heval. destruct k; auto.
-Qed.
-
-Lemma eval_app_inv :
-  forall L P k' pc e t1 t2 a,
-    eval L P pc e (TApp t1 t2) (S k') a ->
-    exists e1' t1' l1 a2 a3,
-      eval L P pc e t1 k' (Atom (VClos e1' t1') l1) /\
-      eval L P pc e t2 k' a2 /\
-      eval L P l1 (a2 :: e1') t1' k' a3 /\
-      a = a3.
-Proof.
-  Admitted.
-
-Lemma eval_decl_inv :
-  forall L P k' pc e t1 t2 a,
-    eval L P pc e (TDecl t1 t2) (S k') a ->
-    exists e1' t1' l1 a2 v3 l3,
-      eval L P pc e t1 k' (Atom (VClos e1' t1') l1) /\
-      eval L P pc e t2 k' a2 /\
-      eval L P l1 (a2 :: e1') t1' k' (Atom v3 l3) /\
-      (l3 = Bottom2 /\
-       a = Atom v3 Bottom2 \/
-       l3 = Top2 /\
-       (forall a2' e2' v3',
-          env_LPequiv L P (a2 :: e1') (a2' :: e2') ->
-          eval L P l1 (a2' :: e2') t1' k' (Atom v3' Top2) ->
-          value_LPequiv L P v3 v3') /\
-       a = Atom v3 Bottom2).
-Proof.
-  Admitted.
