coq/two/LambdaTwoNI.v
@@ -4,6 +4,66 @@ Require Import LibTactics.
 
 Section NI.
 
+Lemma non_interference_nat :
+  forall L P k pc e1 e2 n a1 a2,
+    env_LPequiv L P e1 e2 ->
+    eval L P pc e1 (TNat n) k a1 ->
+    eval L P pc e2 (TNat n) k a2 ->
+    (forall x, P x x) ->
+    atom_LPequiv L P a1 a2.
+Proof.
+  introv He Heval1 Heval2 Prefl.
+  destruct k;
+    (destruct L; destruct pc;
+     simpl in Heval1; simpl in Heval2; subst; [
+       right; left; auto |
+       left; auto |
+       right; right; auto |
+       right; right; auto
+     ]).
+Qed.
+
+Lemma non_interference_var :
+  forall L P k pc e1 e2 n a1 a2,
+    env_LPequiv L P e1 e2 ->
+    eval L P pc e1 (TVar n) k a1 ->
+    eval L P pc e2 (TVar n) k a2 ->
+    (forall x, P x x) ->
+    atom_LPequiv L P a1 a2.
+Proof.
+  introv He Heval1 Heval2 Prefl.
+  destruct k;
+    simpl in Heval1; simpl in Heval2;
+    destruct Heval1 as [v1 Heval1]; destruct Heval1 as [l1 Heval1];
+    destruct Heval2 as [v2 Heval2]; destruct Heval2 as [l2 Heval2];
+    destruct_conjs; subst;
+    assert (Ha: atom_LPequiv L P (Atom v1 l1) (Atom v2 l2)) by
+        (eapply list_forall2_atIndex; eauto);
+    assert (l2 = l1) by
+        (apply atom_LPequiv_lab_inv in Ha; auto);
+    destruct pc; destruct l1; subst; auto;
+    apply atom_LPequiv_raise; assumption.
+Qed.
+
+Lemma non_interference_abs :
+  forall L P k pc e1 e2 t a1 a2,
+    env_LPequiv L P e1 e2 ->
+    eval L P pc e1 (TAbs t) k a1 ->
+    eval L P pc e2 (TAbs t) k a2 ->
+    (forall x, P x x) ->
+    atom_LPequiv L P a1 a2.
+Proof.
+  introv He Heval1 Heval2 Prefl.
+  destruct k;
+    (simpl in Heval1; simpl in Heval2;
+     destruct L; destruct pc; subst; [
+       right; left; auto |
+       left; auto |
+       right; right; auto |
+       right; right; auto
+     ]).
+Qed.
+  
 Theorem non_interference_strong_observer :
   forall L P k pc e1 e2 t a1 a2,
     env_LPequiv L P e1 e2 ->
@@ -14,111 +74,86 @@ Theorem non_interference_strong_observer :
 Proof.
   introv He Heval1 Heval2 Prefl.
   gen pc e1 e2 t a1 a2. 
-  induction k as [| k']; intros; destruct t; auto.
-  - (* E_Nat *)
-    apply eval_nat_inv in Heval1.
-    apply eval_nat_inv in Heval2.
-    destruct L; destruct pc; subst.
-    + right. left. auto.
-    + left. auto.
-    + right. right. auto.
-    + right. right. auto.
-  - (* E_Var *)
-    apply eval_var_inv in Heval1.
-    apply eval_var_inv in Heval2.
-    destruct Heval1 as [v1 Heval1];
-      destruct Heval1 as [l1 Heval1].
-    destruct Heval2 as [v2 Heval2];
-      destruct Heval2 as [l2 Heval2].
-    destruct_conjs; subst.
-    assert (Ha: atom_LPequiv L P (Atom v1 l1) (Atom v2 l2)) by
-        (eapply list_forall2_atIndex; eauto).
-    assert (l2 = l1) by
-        (apply atom_LPequiv_lab_inv in Ha; auto).
-    destruct pc; subst.
-    + rewrite join_bot. assumption.
-    + rewrite join_top. destruct l1; auto.
-      apply atom_LPequiv_raise; assumption.
-  - (* E_Abs *)
-    apply eval_abs_inv in Heval1.
-    apply eval_abs_inv in Heval2.
-    destruct L; destruct pc; subst.
-    + right. left. auto.
-    + left. auto.
-    + right. right. auto.
-    + right. right. auto.
-  - (* E_App *)
-    rename a1 into a. rename a2 into a'.
-    rename e1 into e. rename e2 into e'.
-    apply eval_app_inv in Heval1.
-    apply eval_app_inv in Heval2.
-    destruct Heval1 as [e1' Heval1];
-      destruct Heval1 as [t1' Heval1];
-      destruct Heval1 as [l1 Heval1];
-      destruct Heval1 as [a2 Heval1];
-      destruct Heval1 as [a3 Heval1].
-    destruct Heval2 as [e2' Heval2];
-      destruct Heval2 as [t2' Heval2];
-      destruct Heval2 as [l2 Heval2];
-      destruct Heval2 as [a2' Heval2];
-      destruct Heval2 as [a3' Heval2].
-    destruct_conjs; subst.
-    remember (Atom (VClos e1' t1') l1) as a1.
-    remember (Atom (VClos e2' t2') l2) as a1'.
-    assert (IH1: atom_LPequiv L P a1 a1') by
-        (eapply IHk'; eauto).
-    assert (l2 = l1) by
-        (subst; apply atom_LPequiv_lab_inv in IH1; auto).
-    assert (t2' = t1' /\ env_LPequiv L P e1' e2') by
-        (split; subst; destruct IH1; destruct H2; destruct_conjs; auto).
-    destruct_conjs; subst.
-    assert (IH2: atom_LPequiv L P a2 a2') by
-        (apply (IHk' pc e e' He t2); auto).
-    assert (env_LPequiv L P (a2 :: e1') (a2' :: e2')) by
-        (split; auto).
-    eapply IHk'; eauto.
-  - (* E_Decl *)
-    rename a1 into a. rename a2 into a'.
-    rename e1 into e. rename e2 into e'.
-    apply eval_decl_inv in Heval1.
-    apply eval_decl_inv in Heval2.
-    destruct Heval1 as [e1' Heval1];
-      destruct Heval1 as [t1' Heval1];
-      destruct Heval1 as [l1 Heval1];
-      destruct Heval1 as [a2 Heval1];
-      destruct Heval1 as [v3 Heval1];
-      destruct Heval1 as [l3 Heval1].
-    destruct Heval2 as [e2' Heval2];
-      destruct Heval2 as [t2' Heval2];
-      destruct Heval2 as [l2 Heval2];
-      destruct Heval2 as [a2' Heval2];
-      destruct Heval2 as [v3' Heval2];
-      destruct Heval2 as [l3' Heval2].
-    destruct_conjs.
-    remember (Atom (VClos e1' t1') l1) as a1.
-    remember (Atom (VClos e2' t2') l2) as a1'.
-    assert (IH1: atom_LPequiv L P a1 a1') by
-        (eapply IHk'; eauto).
-    assert (l2 = l1) by
-        (subst; apply atom_LPequiv_lab_inv in IH1; auto).
-    assert (t2' = t1' /\ env_LPequiv L P e1' e2') by
-        (split; subst; destruct IH1; destruct H7; destruct_conjs; auto).
-    destruct_conjs; subst.
-    assert (IH2: atom_LPequiv L P a2 a2') by
-        (apply (IHk' pc e e' He t2); auto).
-    assert (env_LPequiv L P (a2 :: e1') (a2' :: e2')) by
-        (split; auto).
-    assert (IH3: atom_LPequiv L P (Atom v3 l3) (Atom v3' l3')) by
-        (eapply IHk'; eauto).
-    assert (l3' = l3) by
-        (apply atom_LPequiv_lab_inv in IH3; auto). subst.
-    destruct l3; destruct H6; destruct H2; destruct_conjs; 
-    inversion H2; inversion H6; subst; auto.
-    assert (value_LPequiv L P v3 v3') by
-        (eapply H11; eauto).
-    destruct L.
-    + right. left. auto.
-    + right. right. auto.
+  induction k as [| k']; intros.
+  - destruct t; auto.
+    + eapply non_interference_nat; eauto.
+    + eapply non_interference_var; eauto.
+    + eapply non_interference_abs; eauto.
+  - destruct t.
+    + eapply non_interference_nat; eauto.
+    + eapply non_interference_var; eauto.
+    + eapply non_interference_abs; eauto.
+    + (* E_App *)
+      rename a1 into a. rename a2 into a'.
+      rename e1 into e. rename e2 into e'.
+      simpl in Heval1;
+        destruct Heval1 as [e1' Heval1];
+        destruct Heval1 as [t1' Heval1];
+        destruct Heval1 as [l1 Heval1];
+        destruct Heval1 as [a2 Heval1];
+        destruct Heval1 as [a3 Heval1].
+      simpl in Heval2;
+        destruct Heval2 as [e2' Heval2];
+        destruct Heval2 as [t2' Heval2];
+        destruct Heval2 as [l2 Heval2];
+        destruct Heval2 as [a2' Heval2];
+        destruct Heval2 as [a3' Heval2].
+      destruct_conjs; subst.
+      remember (Atom (VClos e1' t1') l1) as a1.
+      remember (Atom (VClos e2' t2') l2) as a1'.
+      assert (IH1: atom_LPequiv L P a1 a1') by
+          (eapply IHk'; eauto).
+      assert (l2 = l1) by
+          (subst; apply atom_LPequiv_lab_inv in IH1; auto).
+      assert (t2' = t1' /\ env_LPequiv L P e1' e2') by
+          (split; subst; destruct IH1; destruct H2; destruct_conjs; auto).
+      destruct_conjs; subst.
+      assert (IH2: atom_LPequiv L P a2 a2') by
+          (apply (IHk' pc e e' He t2); auto).
+      assert (env_LPequiv L P (a2 :: e1') (a2' :: e2')) by
+          (split; auto).
+      eapply IHk'; eauto.
+    + (* E_Decl *)
+      rename a1 into a. rename a2 into a'.
+      rename e1 into e. rename e2 into e'.
+      simpl in Heval1; simpl in Heval2.
+      destruct Heval1 as [e1' Heval1];
+        destruct Heval1 as [t1' Heval1];
+        destruct Heval1 as [l1 Heval1];
+        destruct Heval1 as [a2 Heval1];
+        destruct Heval1 as [v3 Heval1];
+        destruct Heval1 as [l3 Heval1].
+      destruct Heval2 as [e2' Heval2];
+        destruct Heval2 as [t2' Heval2];
+        destruct Heval2 as [l2 Heval2];
+        destruct Heval2 as [a2' Heval2];
+        destruct Heval2 as [v3' Heval2];
+        destruct Heval2 as [l3' Heval2].
+      destruct_conjs.
+      remember (Atom (VClos e1' t1') l1) as a1.
+      remember (Atom (VClos e2' t2') l2) as a1'.
+      assert (IH1: atom_LPequiv L P a1 a1') by
+          (eapply IHk'; eauto).
+      assert (l2 = l1) by
+          (subst; apply atom_LPequiv_lab_inv in IH1; auto).
+      assert (t2' = t1' /\ env_LPequiv L P e1' e2') by
+          (split; subst; destruct IH1; destruct H7; destruct_conjs; auto).
+      destruct_conjs; subst.
+      assert (IH2: atom_LPequiv L P a2 a2') by
+          (apply (IHk' pc e e' He t2); auto).
+      assert (env_LPequiv L P (a2 :: e1') (a2' :: e2')) by
+          (split; auto).
+      assert (IH3: atom_LPequiv L P (Atom v3 l3) (Atom v3' l3')) by
+          (eapply IHk'; eauto).
+      assert (l3' = l3) by
+          (apply atom_LPequiv_lab_inv in IH3; auto). subst.
+      destruct l3; subst; auto.
+      destruct_conjs; subst.
+      assert (value_LPequiv L P v3 v3') by
+          (eapply H6; eauto).
+      destruct L.
+      * right. left. auto.
+      * right. right. auto.
 Qed.
 
 Theorem non_interference :
